## 시간 복잡도

<br>

- 재귀식을 `0() notation` 수준으로 풀기

  <br>

  - **T(n) = T(n-1) + 1, T(0) = 1 **

    ```
     T(n)  = T(n-1) + 1
    T(n-1) = T(n-2) + 1
    T(n-2) = T(n-3) + 1
    
     T(n)  = T(n-3) + 1 + 1 + 1
     T(n)  = T(n-K) + K
     T(n)  = T(0) + n
    	   = n + 1
    	   
    >>> O(N)
    ```

  <br>

  - **T(n) = T(n-1) + n, T(0) = 1**

    ```
     T(n)  = T(n-1) + n
    T(n-1) = T(n-2) + n-1
    T(n-2) = T(n-3) + n-2
    
     T(n)  = T(n-3) + n-2 + n-1 + n
     T(n)  = T(n-3) + 3n-3
     T(n)  = T(n-k) + k(n-1)
     T(n)  = T(0) + n(n-1)
           = n^2 - n + 1
    
    >>> O(N^2)
    ```

  <br>

  - **T(n) = T(n-1) + logn, T(0) = 1**

    ```
     T(n)  = T(n-1) + logn
    T(n-1) = T(n-2) + log(n-1)
    T(n-2) = T(n-3) + log(n-2)
    
     T(n)  = T(n-3) + log((n-2)(n-1)n)
     T(n)  = T(n-k) + log( n * (n-1) * (n-2) * ... * (n-(k-1)) )
     T(n)  = T(n-n) + log( n * (n-1) * (n-2) * ... * (n-(n-1)) )
     T(n)  = T(n-n) + log( n * (n-1) * (n-2) * ... * 1 )
           = 1 + log(n!) <= 1 + long(n^n)
           = 1 + nlogn
           
    >>> O(nlogn)
    ```

  <br>

  - **T(n) = T(n/2) + 1**

    ```
     T(n)  = T(n/2) + 1
    T(n/2) = T(n/4) + 1
    T(n/4) = T(n/8) + 1
    
     T(n)  = T(n/2^k) + k
     T(n)  = T(n/2^longn) + logn
     T(n)  = T(n/n) + logn
           = T(1) + logn
    
    >>> O(logn)
    ```

  <br>

  - **T(n) = T(n/2) + n, T(1) = 1**

    ```
     T(n)  = T(n/2) + n
    T(n/2) = T(n/4) + n/2
    T(n/4) = T(n/8) + n/4
    
     T(n)  = T(n/2) + n
           = T(n/4) + n/2 + n
           = T(n/8) + n + n/2 + n/4
           = T(n/2^k) + n( 1 + 1/2 + ... + 1/2^(k-1) ) # 등비수열의 합은 1
           = T(1) + n(1 + 1)
           = 1 + 2n
    
    >>> O(n)
    ```

  <br>

  - **T(n) = 2T(n/2) + n, T(1) = 1**

    ```
     T(n)  = 2T(n/2) + n
    T(n/2) = 2T(n/4) + n/2
    T(n/4) = 2T(n/8) + n/4
    
     T(n)  = 2T(n/2) + n
     T(n)  = 2(2T(n/4) + n/2) + n
     T(n)  = 2(2(2T(n/8) + n/4) + n/2) + n
     
     T(n)  = 8T(n/8) + n + n + n
           = 8T(n/8) + 3n
           = 2^kT(n/2^k) + kn
           = nT(1) + nlogn
           = n + nlogn
           = n(log2 + logn)
           = nlog(2n)
           
    >>> O(nlogn)
    ```

  <br>

  - **T(n) = 3T(n/2) + n, T(1) = 1**

    ```
     T(n)  = 3T(n/2) + n
    T(n/2) = 3T(n/4) + n/2
    T(n/4) = 3T(n/8) + n/4
    
     T(n)  = 3(3T(n/4) + n/2) + n
           = 3(3(3T(n/8) + n/4) + n/2) + n
           = 27T(n/8) + 9n/4 + 3n/2 + n
           
     T(n)  = 3^kT(n/2^k) + n(3/2)^(k-1) + n(3/2)^(k-2) + n
           = ...
           
    >>> O(n^(log2(3)))
    ```

<br>

<br>

## 재귀

<br>

- **피보나치 수열**

  - 정확성 증명

    ```
    F(n) = F(n-1) + F(n-2)  / F(1) = 1
    
    F(k) = F(k-1) + F(k-2) 가 성립한다고 가정할때,  F(k+1) = F(k) + F(k-1) 가 성립합을 보인다. 
    
    F(k) = F(k-1) + F(k-2)
    F(k) + F(k-1) = F(k-1) + F(k-2) + F(k-1)
                  = F(k-1) + F(k)
                  = F(k+1)
    
    >>> F(k+1) = F(k) + F(k-1)
    ```

  <br>

  - 시간복잡도

    ```
     T(n)  = T(n-1) + T(n-2) + 1  <  T(n-1) + T(n-1) + 1
    
    T(n-1) = 2T(n-2) + 1
    T(n-2) = 2T(n-3) + 1
    
     T(n)  = 2T(n-1) + 1
           = 2(2T(n-2)) + 1
           = 2(2(2T(n-3) + 1) + 1) + 1
           = 2^3T(n-3) + 4 + 2 + 1
           = 2^kT(n-k) + 2^0 + 2^1 + ... + 2^(k-1)
           = 2^nT(n-n) + 2^0 + 2^1 + ... + 2^(n-1)
           = 2^nT(0) + 2^n - 1
    
    >>> O(2^n)
    ```

    